work on bedrock2Examples involving leakage (including using the fancy new notations!)

bedrock2/src/bedrock2Examples/ct.v
@@ -20,27 +20,23 @@ Import LeakageProgramLogic.Coercions.
 Section WithParameters.
   Context {word: word.word 32} {mem: Interface.map.map word Byte.byte}.
   Context {word_ok : word.ok word} {mem_ok : Interface.map.ok mem}.
-  Context {pick_sp: PickSp}.
+  Context {pick_sp: PickSp}. Locate "fnspec!".
 
 #[global] Instance ctspec_of_div3329 : spec_of "div3329" :=
-  fun functions => forall k, exists k_, forall t m x,
-      LeakageWeakestPrecondition.call functions "div3329" k t m [x]
-        (fun k' t' m' rets => exists ret, rets = [ret]
-        /\ t' = t /\ m' = m /\ k' = k_
-        (*x < 2^32 -> ret = x / 3329 :> Z*) ).
+    fnspec_ex! f "div3329" x ~> ret,
+      { requires k t m := True ; ensures k' t' m' := t' = t /\ m' = m /\ k' = f k }.
 
 Lemma div3329_ct : program_logic_goal_for_function! div3329.
 Proof.
   repeat (straightline || eexists).
-  { (* no leakag -- 3 minutes *) cbv [k' k'0]. cbn. exact eq_refl. }
+  { (* no leakag -- 3 minutes *) cbn. exact eq_refl. }
 Qed.
 
 #[global] Instance vtspec_of_div3329 : spec_of "div3329_vartime" :=
-  fun functions => forall k, forall t m x,
-      LeakageWeakestPrecondition.call functions "div3329_vartime" k t m [x]
-        (fun k' t' m' rets => exists ret, rets = [ret]
-        /\ t' = t /\ m' = m /\ k' = [leak_word (word.of_Z 3329); leak_word x]++k
-        (*x < 2^32 -> ret = x / 3329 :> Z*) ).
+  fnspec! "div3329_vartime" x ~> ret,
+    { requires k t m := True ;
+      ensures k' t' m' := t' = t /\ m' = m /\
+                            k' = [leak_word (word.of_Z 3329); leak_word x]++k }.
 
 Lemma div3329_vt : program_logic_goal_for_function! div3329_vartime.
 Proof.
@@ -53,10 +49,10 @@ Import Byte.
 Definition getchar_event c : LogItem :=
   ((Interface.map.empty, "getchar", []), (Interface.map.empty, [word.of_Z (byte.unsigned c)])).
 #[global] Instance ctspec_of_getchar : spec_of "getchar" :=
-  fun functions => exists f, forall k t m,
-      LeakageWeakestPrecondition.call functions "getchar" k t m []
-        (fun k' t' m' rets => exists c, rets = [word.of_Z (byte.unsigned c)] /\ k' = f ++ k /\ m' = m /\
-        t' = cons (getchar_event c) t ).
+  fnspec_ex! f "getchar" ~> ret,
+    { requires k t m := True ; ensures k' t' m' :=
+        exists c, ret = word.of_Z (byte.unsigned c) /\
+               k' = f ++ k /\ m' = m /\ t' = cons (getchar_event c) t }.
 
 Definition getline := func! (dst, n) ~> n {
   i = $0;
@@ -85,16 +81,15 @@ Local Fixpoint getline_leakage f dst n (bs : nat) (i : word) :=
   end.
 
 #[global] Instance ctspec_of_getline : spec_of "getline" :=
-  fun functions => exists f, forall k (dst n : word) d t m R,
-  (d$@dst * R) m -> length d = n :> Z ->
-      LeakageWeakestPrecondition.call functions "getline" k t m [dst; n]
-        (fun k' t' m' rets => exists bs es l, rets = [l] /\ k' = f dst n l ++ k /\
+  fnspec_ex! f "getline" (dst n : word) / d R ~> l,
+    { requires k t m := (d$@dst * R) m /\ length d = n :> Z ;
+      ensures k' t' m' := exists bs es,
+        k' = f dst n l ++ k /\
         (bs$@dst * es$@(word.add dst l) * R) m' /\
         length bs = l :> Z /\
         length bs + length es = n :> Z /\
         t' = getline_io n bs ++ t 
-        (* /\ ~ In Byte.x0a bs *)
-        ).
+        (* /\ ~ In Byte.x0a bs *) }.
 
 (* Mon Jul  1 14:24:28 EDT 2024 *)
 
@@ -103,7 +98,7 @@ Import Separation SeparationLogic.
 
 Lemma getline_ct : program_logic_goal_for_function! getline.
 Proof.
-  enter getline. destruct H as [f H]. Print straightline.
+  enter getline. destruct H as [f H].
   intros;
          match goal with
          | |- call _ _ _ _ _ _ _ => idtac
@@ -146,8 +141,8 @@ Proof.
          PrimitivePair.pair._1 PrimitivePair.pair._2] in *;
     repeat straightline.
     { eapply Z.gt_wf. }
-    { split. { subst v. rewrite word.unsigned_of_Z_0. blia. }
-      subst v; rewrite word.add_0_r; split; [ecancel_assumption|]. rewrite word.sub_0_r; auto. }
+    { split. { subst i. rewrite word.unsigned_of_Z_0. blia. }
+      subst i; rewrite word.add_0_r; split; [ecancel_assumption|]. rewrite word.sub_0_r; auto. }
 
     { 
       pose proof word.unsigned_range n.
@@ -155,7 +150,7 @@ Proof.
       subst br. rewrite word.unsigned_ltu in H2; case Z.ltb eqn:? in H2; 
           rewrite ?word.unsigned_of_Z_1, ?word.unsigned_of_Z_0, ?word.unsigned_sub_nowrap  in *; try blia; [].
       eapply LeakageWeakestPreconditionProperties.Proper_call; repeat intro; cycle 1.
-      { eapply H. }
+      { eapply H. exact I. }
       repeat straightline.
       eexists _, _; repeat straightline.
       split; repeat straightline.
@@ -172,15 +167,15 @@ Proof.
           split. { rewrite word.unsigned_sub_nowrap; blia. }
           split. { blia. }
           split. { (* I/O *)
-            cbv [getline_io]. cbn [map rev List.app length]. case (Z.eqb_spec (n-x3) 0%nat) as []; try blia.
+            cbv [getline_io]. cbn [map rev List.app length]. case (Z.eqb_spec (n'0-x3) 0%nat) as []; try blia.
             rewrite app_nil_r. subst a0. simpl.
             eapply f_equal2; f_equal; trivial.
             progress change 10 with (byte.unsigned Byte.x0a) in H4.
-            pose proof byte.unsigned_range x1.
+            pose proof byte.unsigned_range x2.
             pose proof byte.unsigned_range Byte.x0a.
             eapply word.of_Z_inj_small, byte.unsigned_inj in H4; trivial; blia. }
           (* leakage *)
-          subst k'. subst k'''. cbn [getline_leakage leak_binop "++" length].
+          subst k'''. cbn [getline_leakage leak_binop "++" length].
           rewrite (proj2 (Z.eqb_neq _ _)) by blia; trivial. simpl. rewrite <- app_assoc. reflexivity. } }
 
       (* store *)
@@ -190,7 +185,7 @@ Proof.
       right; repeat straightline.
       eexists _, _, _; repeat straightline.
       { instantiate (1:=x).
-        subst v3.
+        subst i.
         rewrite word.add_assoc.
         split. { rewrite word.unsigned_add_nowrap; rewrite ?word.unsigned_of_Z_1; try blia. }
         split; [ecancel_assumption|].
@@ -200,22 +195,22 @@ Proof.
         pose proof word.unsigned_sub_nowrap n (word.add x3 (word.of_Z 1)).
         blia. }
       { split.
-        { subst  v3.
+        { subst i.
           pose proof word.unsigned_of_Z_1.
           pose proof word.unsigned_add_nowrap x3 (word.of_Z 1).
           pose proof word.unsigned_sub_nowrap n (word.add x3 (word.of_Z 1)).
           blia. }
         repeat straightline.
         (* subroutine return *)
-        subst v3.
+        subst i.
 
         rename x9 into bs.
         rename x10 into es.
-        rename x5 into I.
+        rename x6 into I.
         rename x3 into _i.
         rewrite word.add_assoc in H10.
 
-        eexists (byte.of_Z v2::bs), (es).
+        eexists (byte.of_Z x1 :: bs), (es).
         cbn ["$@" "++"].
         split. { ecancel_assumption. }
         split; trivial.
@@ -241,11 +236,11 @@ Proof.
           cbn [map List.app].
           f_equal.
           f_equal.
-          subst v2.
-          pose proof byte.unsigned_range x1.
+          subst x1.
+          pose proof byte.unsigned_range x2.
           rewrite word.unsigned_of_Z_nowrap, byte.of_Z_unsigned; trivial; blia. }
         (* leakage *)
-        subst K k'0 k'' k' a1; cbn [getline_leakage leak_binop length].
+        subst K a1; cbn [getline_leakage leak_binop length].
         rewrite (proj2 (Z.eqb_neq _ _)) by blia; trivial.
         repeat (simpl || rewrite <- app_assoc). reflexivity. } }
 
@@ -265,9 +260,9 @@ Proof.
       destruct x; try (cbn in *; blia).
       cbn [getline_leakage length]; rewrite Z.eqb_refl; trivial. }
 
-    split. { subst k0 v0 v. rewrite word.sub_0_r in *.
+    do 2 eexists. split. { subst k0 i. rewrite word.sub_0_r in *.
       assert (length x3 = Z.to_nat (word.unsigned x0)) as -> by blia. reflexivity. }
-    subst v.
+    subst i.
     rewrite word.add_0_r in *.
     split.
     { ecancel_assumption. }
@@ -291,21 +286,16 @@ Definition password_checker := func! (password) ~> ret {
                                    unpack! ok = memequal(x, password, $8);
                                    ret = (n == $8) & ok
                                  }.
-Print getline_io.
 
 #[global] Instance ctspec_of_password_checker : spec_of "password_checker" :=
-  fun functions => exists f, forall (username password_addr : word), forall R t m password,
-      length password = 8 :> Z ->
-      (password$@password_addr * R) m ->
-      LeakageWeakestPrecondition.call functions "password_checker" [] t m [password_addr]
-        (fun k' t' m' rets =>
-           exists bs ret (l : word),
-             rets = [ret (*bs =? password*)] /\
-               (password$@password_addr * R) m' /\
-               t' = getline_io 8 bs ++ t /\
-               length bs = l :> Z /\
-               (k' = f password_addr l) /\
-               (word.unsigned ret = 1 <-> bs = password)).
+  fnspec_ex! f "password_checker" password_addr / R password ~> ret (*bs =? password*),
+    { requires k t m := length password = 8 :> Z /\ (password$@password_addr * R) m ;
+      ensures k' t' m' := exists bs (l : word),
+        (password$@password_addr * R) m' /\
+          t' = getline_io 8 bs ++ t /\
+          length bs = l :> Z /\
+          (k' = f k password_addr l) /\
+          (word.unsigned ret = 1 <-> bs = password) }.
 
 Fail Lemma password_checker_ct : program_logic_goal_for_function! password_checker. (*Why*)
 Global Instance spec_of_memequal : spec_of "memequal" := spec_of_memequal.
@@ -328,7 +318,7 @@ Proof.
   
   repeat straightline.
   eapply LeakageWeakestPreconditionProperties.Proper_call; repeat intro; cycle 1.
-  { eapply H. 2: rewrite word.unsigned_of_Z; eassumption. ecancel_assumption. }
+  { eapply H. split. 2: rewrite word.unsigned_of_Z; eassumption. ecancel_assumption. }
   repeat straightline.
   seprewrite_in_by @Array.bytearray_index_merge H9 ltac:(blia).
   eapply LeakageWeakestPreconditionProperties.Proper_call; repeat intro; cycle 1.
@@ -338,44 +328,39 @@ Proof.
     split.
     { rewrite ?app_length; blia. }
     { rewrite H1. rewrite word.unsigned_of_Z. reflexivity. } }
-  assert (length ((x ++ x0)) = 8%nat).
+  assert (length ((x0 ++ x1)) = 8%nat).
   { rewrite ?app_length. rewrite word.unsigned_of_Z_nowrap in H11; blia. }
   repeat straightline.
-  split. { ecancel_assumption. }
+  do 2 eexists. split. { ecancel_assumption. }
   split. { subst a0. rewrite word.unsigned_of_Z. exact eq_refl. }
   split. { eassumption. }
   split. { (* leakage *)
-    subst a0. subst a. subst k'0. subst k'. reflexivity. }
+    subst a0. subst a. subst a2. instantiate (1 := fun _ _ => _). simpl. reflexivity. }
   { (* functional correctness *)
-    subst v.
-    destruct (word.eqb_spec x1 (word.of_Z 8)) as [->|?]; cycle 1.
+    subst ret.
+    destruct (word.eqb_spec x (word.of_Z 8)) as [->|?]; cycle 1.
     { rewrite word.unsigned_and_nowrap, word.unsigned_of_Z_0, Z.land_0_l; split; try discriminate.
       intros X%(f_equal (@length _)). case H13; clear H13; apply word.unsigned_inj.
       rewrite <-H10, X, word.unsigned_of_Z_nowrap; blia. }
     rewrite word.unsigned_and_nowrap, word.unsigned_of_Z_1.
-    destruct x0; cycle 1.
-    { cbn [length] in *. rewrite word.unsigned_of_Z_nowrap in H10, H11; blia. }
-    { rewrite ?app_nil_r in *. rewrite <-H16.
+    destruct x1; cycle 1.
+    { cbn [length] in *. blia. }     { rewrite ?app_nil_r in *. rewrite <-H16.
       case H15 as [->|]; intuition try congruence. rewrite H15. trivial. } }
-  Unshelve.
-  all: assumption || exact nil.
 Qed.
 
 Definition output_event x : LogItem :=
   ((Interface.map.empty, "output", [x]), (Interface.map.empty, [])).
 #[global] Instance ctspec_of_output : spec_of "output" :=
-  fun functions => exists f, forall k t m x,
-      LeakageWeakestPrecondition.call functions "output" k t m [x]
-        (fun k' t' m' rets => rets = [] /\ k' = f ++ k /\ m' = m /\
-        t' = cons (output_event x) t ).
+  fnspec_ex! f "output" x,
+    { requires k t m := True ;
+      ensures k' t' m' := k' = f ++ k /\ m' = m /\ t' = cons (output_event x) t }.
 
 Definition getprime_event p : LogItem :=
   ((Interface.map.empty, "getprime", []), (Interface.map.empty, [p])).
 #[global] Instance ctspec_of_getprime : spec_of "getprime" :=
-  fun functions => exists f, forall k t m,
-      LeakageWeakestPrecondition.call functions "getprime" k t m []
-        (fun k' t' m' rets => exists p, rets = [p] /\ k' = f ++ k /\ m' = m /\
-        t' = cons (getprime_event p) t ).
+  fnspec_ex! f "getprime" ~> p,
+    { requires k t m := True ;
+      ensures k' t' m' := k' = f ++ k /\ m' = m /\ t' = cons (getprime_event p) t }.
 
 Definition semiprime := func! () ~> (p, q) {
   unpack! p = getprime();
@@ -385,10 +370,11 @@ Definition semiprime := func! () ~> (p, q) {
 }.
 
 #[global] Instance ctspec_of_semiprime : spec_of "semiprime" :=
-  fun functions => exists f, forall t m k,
-      LeakageWeakestPrecondition.call functions "semiprime" k t m []
-      (fun k' t' m' rets => exists p q, rets = [p;q] /\ k' = f ++ k /\ m' = m
-        /\ t' = [output_event (word.mul p q); getprime_event q; getprime_event p]++t).
+  fnspec_ex! f "semiprime" ~> p q,
+    { requires k t m := True ;
+      ensures k' t' m' :=
+        k' = f ++ k /\ m' = m
+        /\ t' = [output_event (word.mul p q); getprime_event q; getprime_event p]++ t }.
 
 Lemma semiprime_ct : program_logic_goal_for_function! semiprime.
 Proof.
@@ -407,7 +393,7 @@ Proof.
   eapply LeakageWeakestPreconditionProperties.Proper_call; repeat intro; [|eapply H]; repeat straightline.
   eapply LeakageWeakestPreconditionProperties.Proper_call; repeat intro; [|eapply H]; repeat straightline.
   eapply LeakageWeakestPreconditionProperties.Proper_call; repeat intro; [|eapply H1]; repeat straightline.
-  Tactics.ssplit; trivial; align_trace.
+  Tactics.ssplit; trivial; simpl in *; align_trace.
 Qed.
 
 Definition maskloop := func! (a) {
@@ -420,7 +406,6 @@ Definition maskloop := func! (a) {
 }.
 
 Require Import coqutil.Map.Interface bedrock2.Map.Separation bedrock2.Map.SeparationLogic.
-
 
 (*#[global] Instance ctspec_of_maskloop : spec_of "maskloop" :=
   fun functions => forall k a, exists k_, forall a0 a1 R t m,
@@ -454,3 +439,4 @@ Proof.
     left; Tactics.ssplit; trivial; ecancel_assumption. }
   intuition subst.
 Abort.*)
+End WithParameters.
